Foundation/FirstOrder/Arithmetic/ISigma1/Prenex.lean
@@ -18,18 +18,18 @@ namespace LO.FirstOrder.Arithmetic.ISigma1
 
 variable {n : ℕ}
 
-lemma nonempty_strictEquiv {φ : ArithmeticSemisentence n} (h : Hierarchy 𝚺 1 φ) :
-    Nonempty (StrictEquiv 𝗜𝚺₁ 𝚺 1 φ) :=
-  Arithmetic.nonempty_strictEquiv h inferInstance
+lemma nonempty_strictHierarchyFormulaEquivOf {φ : ArithmeticSemisentence n} (h : Hierarchy 𝚺 1 φ) :
+    Nonempty (StrictHierarchyFormulaEquivOf 𝗜𝚺₁ 𝚺 1 φ) :=
+  Arithmetic.nonempty_strictHierarchyFormulaEquivOf h inferInstance
 
 lemma exists_strictHierarchy_provable {φ : ArithmeticSemisentence n} (h : Hierarchy 𝚺 1 φ) :
     ∃ θ : ArithmeticSemisentence (n + 1), Hierarchy 𝚺 0 θ ∧ 𝗜𝚺₁ ⊢ ∀¹* (φ 🡘 ∃¹ θ) := by
-  have ⟨⟨ψ, ψ_hie, ψ_iff⟩⟩ := nonempty_strictEquiv h;
-  obtain ⟨θ, rfl, hθ⟩ := ψ_hie.sigma_succ_elim;
-  use θ;
+  obtain ⟨W⟩ := nonempty_strictHierarchyFormulaEquivOf h;
+  use (↑W.sigmaInv : ArithmeticSemisentence (n + 1));
   and_intros;
-  . exact StrictHierarchy.zero_iff.mp hθ;
-  . assumption;
+  . exact W.sigmaInv.deltaZero;
+  . rw [← W.coe_sigmaInv];
+    exact W.provable;
 
 lemma exists_strictHierarchy_provable_of_sentence {σ : ArithmeticSentence} (h : Hierarchy 𝚺 1 σ) :
     ∃ θ : ArithmeticSemisentence 1, Hierarchy 𝚺 0 θ ∧ 𝗜𝚺₁ ⊢ σ 🡘 ∃¹ θ :=
